---
title: "APM1111 FA2"
author: "DESQUITADO, Yuichi P."
date: "2023-09-17"
output: html_document
---

### 3.49 Prove that $\sum_{j=1}^{N}{(X_j - 1)^2} = \sum_{j=1}^{N}{X_j^2} - 2\sum_{j=1}^{N}{X_j + N}$.

First, we expand the expression $(X_j-1)^2$.
$$
\sum_{j=1}^{N}{(X_j-1)^2}=\sum_{j=1}^{N}{X_j^2 - 2X_j + 1}
$$

By the summation rule, we can get the summation of a function by adding the summation of the terms.

$$
\sum_{j=1}^{N}{X_j^2 - 2X_j + 1} = \sum_{j=1}^{N}{X_j^2} - 2\sum_{j=1}^{N}{X_j} + \sum_{j=1}^{N}{1}
$$

We can simplify $\sum_{j=1}^{N}{1} = N$ as $1 + 1 + 1 +...+N=N$. Therefore, we get:

$$
\sum_{j=1}^{N}{(X_j-1)^2} = \sum_{j=1}^{N}{X_j^2} - 2\sum_{j=1}^{N}{X_j} + N
$$

---

### 3.51 Two variables, $U$ and $V$, assume the values $U_1 = 3$, $U_2 = -2$, $U_3 = 5$, and $V_1 = -4$, $V_2 = -1$, $V_3 = 6$, respectively. Calculate (a) $\sum{UV}$, (b) $\sum{(U + 3)(V - 4)}$, (c) $\sum{V^2}$, (d) $(\sum{U})(\sum{V})^2$, (e) $\sum{UV^2}$, (f) $\sum{(U^2 - 2V^2 + 2)}$, and (g)$\sum{(U/V)}$.

(a)
$$
\sum_{i=1}^{3}{U_i V_i} = (3)(-4) + (-2)(-1) + (5)(6) = -12 + 2 + 30 = 32 - 12 = 20
$$

(b)
$$
\sum_{i=1}^{3}{(U_i + 3)(V_i - 4)} 
\\ = ((3 + 3)(-4 - 4))+((-2 + 3)(-1 - 4))+((5 + 3)(6 - 4))
\\ =((6)(-8))+((1)(-5))+((8)(2))
\\ = -48-5+16
\\ = 16 - 53
\\ = -37
$$

(c)
$$
\sum_{i=1}^{3}{V_i^2}
\\ = (-4)^2 + (-1)^2 + 6^2
\\ = 16 + 1 + 36
\\ = 53
$$

(d)
$$
(\sum_{i=1}^{3}{U})(\sum_{i=1}^{3}{V})^2
\\ = (3 - 2 + 5)(-4-1+6)^2
\\ = (6)(1)^2
\\ = (6)(1)
\\ = 6
$$

(e)
$$
\sum_{i=1}^{3}{U_iV_i^2}
\\ = ((3)(-4)^2) + ((-2)(-1)^2) + ((5)(6)^2)
\\ = ((3)(16)) + ((-2)(1)) + ((5)(36))
\\ = 48 - 2 + 180
\\ = 228 - 2
\\ = 226
$$

(f)
$$
\sum_{i=1}^{3}{(U_i^2 - 2V_i^2 + 2)} = \sum_{i=1}^{3}{U_i^2} - \sum_{i=1}^{3}{2V_i^2} + \sum_{i=1}^{3}{2} = \sum_{i=1}^{3}{U_i^2} - 2\sum_{i=1}^{3}{V_i^2} + 2N
\\ = (3^2 + (-2)^2 + 5^2) - 2((-4)^2 + (-1)^2 + 6^2) + 2(3)
\\ = (9 + 4 + 25) - 2(16 + 1 + 36) + 6
\\ = 38 - 2(53) + 6
\\ = 44 - 106
\\ = -62
$$

(g)
$$
\sum_{i=1}^{3}{\dfrac{U_i}{V_i}}
\\ = \dfrac{3}{-4} + \dfrac{-2}{-1} + {\dfrac{5}{6}}
\\ = 2 + \dfrac{5}{6} - \dfrac{3}{4}
\\ = \dfrac{24 + 10 - 9}{12}
\\ = \dfrac{34 - 9}{12}
\\ = \dfrac{25}{12} = 2\dfrac{1}{12} = 2.08333...
$$

---

### 3.90 Find the Geometric Mean of the sets (a) 3, 5, 8, 3, 7, 2 and (b) 28.5, 73.6, 47.2, 31.5, 64.8.

(a)
$$
X = 3, 5, 8, 3, 7, 2
N = 6
\\ G = \sqrt[N]{X_1 X_2 ...X_6}
\\ G = \sqrt[6]{(3)(5)(8)(3)(7)(2)}
\\ G = \sqrt[6]{5040} \approx 4.14068
$$

(b)
$$
X = 28.5, 73.6, 47.2, 31.5, 64.8
\\ N = 5
\\ G = \sqrt[5]{(28.5)(73.6)(47.2)(31.5)(64.8)}
\\ G = \sqrt[5]{202092516.864} \approx 45.82580
$$
